## R-Algebra

I have devised a superset of Algebra that surprisingly still keeps one critical rule, x =|x !



R-Algebra can only be used to derive formulas in algebra!



= | stands for R-Algebra, so if there is = | and you can prove that a chain of x = | y works in algebra thats how you can do derivation with R-Algebra.

hard dirac is just a naming scheme for the number 2ei. | = | means something still needs further statements in between, = | is supposed to mean proven up to a reduction to algebra. so if you can fully collapse = | and | = | to each sides of an equation then you possibly have an algebraic derivation iff the result != 0.



## Complex Number Analysis

An Informal Number x from X is a complex number with an imaginary component restricted to R/Q.



scratch work:



[ i 1 | 1 i ] x [ i 1 | 1 i ] = [ 0 2i | 2i 0 ]



then ...



[ i e | e i ] x [ i e | i e ] = [ 0 {hard dirac} | 0 {hard dirac} ]



so ...



-1 + ei =| 0 



e^2 + ei =| {hard dirac} =| 2ei



e^2 - 1 =| x =| 0 



so,



e^i = +/- 1



how,



{hard dirac} =| 0 + 2ei



e^2 =| ei



-1 + ei =| -1 + e^2 =| 0 <=> e^2 =| ei =| 1



0 + 2ei =| e^2 + ei =| 2e^2



=>



e^2 =| +/> 1



## R-Algebra Group Proof



show, e^2 =| +> 1 since e^2 =| ei



<=> e^2 =| 1-1



an informal number is from the set X of informal numbers.



i. e^2 - 1 =| 0 <=> 1*1 =| 0*1 =| 0 <=> 1/0 =| 0

   

   -1 + e^2 =| 0

   

   -1 + 0 =| 0

   

   x =| 0



ii. -1 + ei =| 0 <=> x =| x



iii. e^2 + ei =| 0



1. x =| x



2. x =| 0



3. 1/0 =| 0



## Informal R-Algebra Theory



[ Write Here ]



axiom 1. {hard dirac} =| 0 + 2ei =| e^2 + ei =| +/> 1 + ei =| +/> 2



## R-Calculus



e^2 =| ei =| +> 1 =| 1-1 =| 0  



-< 1 |=| ei (1.)



+> 1 |=| -< 1 (2.)



+> 1 |=| -< 1



+> 2 =| 1 + 1/1 =| 1+1 =| {hard dirac} =| 1-1 =| 1 - 1/1 =|-< 2



+>2 =| 2



+> 1 =| 1



-< 1 =| -1



e^2 =| +> 1



e^2 =| 0



e^2 =| 1-1



e^2 =| -< 1



=>



-< 1 |=| ei (1.)



xei =| +> x =| -< x



## Informal Algebra



e^i = +/- 1 *(1)



e^i*pi + 1 = 0  # eulers identity



(+/- 1)^pi + 1 =| 0



(+/- 1) + 1 =| 0



e^i + 1 =| 0



e^i =| -1



iln(e) = ln(-1)



iln(e) = i*pi # ln(-1) = i*pi



i = i*pi # ln(e) = 1



=>



sqrt(1) = +/- 1 = e^i =| -1



=> 



sqrt(1) + 1 =| 0



sqrt(n*n) + n =| 0 



+/- n + n =| 0



=>



sqrt(-1) = i = i*pi = iln(e) = ln(-1) = ln(e^i)



e^sqrt(-1) = e^i = e^ln(e^i)



=>



sqrt(-n) = sqrt(n)*i = sqrt(n)*ln(e^i)



=> 



e^sqrt(-1) = e^i = +/- 1 = sqrt(1)



sqrt(n) = e^sqrt(-n)



sqrt(n) = e^i*sqrt(n)



=>



sqrt(1/4) = 1/2 



sqrt(-1/4) = e^sqrt(1/4) = e^i*sqrt(-1/4) = +/- sqrt(-1/4) = +/- isqrt(1/4) = +/- i1/2



=>



sqrt(n) = e^sqrt(-n) = e^i*sqrt(n) = +/- sqrt(n)



sqrt(-n) = +/- isqrt(n)



## i hypothesis (i is an irrational number)



e^i = cos(1) + isin(1) = +/- 1 = 0.54030230586 + isin(1)



=>



isin(1) = 0.45969769414 or -1.54030230586 



sin(1) = 0.8414709848



i = 0.45969769414 / 0.8414709848 or -1.54030230586 / 0.8414709848



i = 0.54630248985 or -1.83048772172



## Ordinality of Glider Addition Relations



+/- ln(e) = 2ei = 1 or 2 or 3 = +/> 2



e^i + ei = 1(ln(e)) or 2 or 3 = +/> 2



+/> 0 = 0 or 1 or -1 = (+/> 1)*(0) 



+/> 0 = +/> 1 * 0 = 0 or +/> 0 , since (1)



(*1) x = 0 = x*0 = 0*0 = 0 ! 



thus,



+>x = +/- x or +/- (x-1) or +/- (x+1) or 0
