## Scratch Work

+>1 = ei ERROR

[ i 1 | 1 i ] x [ i 1 | 1 i ] = [ 0 2i | 2i 0 ]
[ i e | e i ] x [ i e | i e ] = [ 0 {hard dirac} | 0 {hard dirac} ]
-1 + ei =| 0
e^2 + ei |= {hard dirac} |=| 2ei
e^2 - 1 |=| x =| 0
e^i = +/- 1 ?
{hard dirac} |=| 0 + 2ei
e^2 =| ei
-1 + ei =| -1 + e^2 =| 0 <=> e^2 =| ei =| 1
0 + 2ei =| e^2 + ei =| 2e^2 =>
e^2 =| +/> 1
show, e^2 =| +> 1 since e^2 =| ei
<=> e^2 =| 1-1
i. e^2 - 1 =| 0 <=> 1*1 =| 0*1 =| 0 <=> 1/0 =| 0
-1 + e^2 =| 0
-1 + 0 =| 0
x =| 0
ii. -1 + ei =| 0 <=> x =| x
iii. e^2 + ei =| 0

1. {hard dirac} =| 0 + 2ei =| e^2 + ei =| +/> 1 + ei =| +/> 2 ERROR
   e^2 =| ei =| +> 1 =| 1-1 =| 0
   -< 1 |=| ei (1.)
   +> 1 |=| -< 1 (2.)
   +> 1 |=| -< 1
   +> 2 =| 1 + 1/1 =| 1+1 =| {hard dirac} =| 1-1 =| 1 - 1/1 =|-< 2
   +>2 =| 2
   +> 1 =| 1
   -< 1 =| -1
   e^2 =| +> 1
   e^2 =| 0
   e^2 =| 1-1
   e^2 =| -< 1 =>
   -< 1 |=| ei (1.)
   xei =| +> x =| -< x
   e^i = +/- 1 \*(1)
   e^i\*pi + 1 = 0 # eulers identity
   (+/- 1)^pi + 1 =| 0
   (+/- 1) + 1 =| 0
   e^i + 1 =| 0
   e^i =| -1
   iln(e) = ln(-1)
   iln(e) = i*pi # ln(-1) = i*pi
   i = i\*pi # ln(e) = 1 =>
   sqrt(1) = +/- 1 = e^i =| -1 =>
   sqrt(1) + 1 =| 0
   sqrt(n\*n) + n =| 0
   +/- n + n =| 0 =>
   sqrt(-1) = i = i\*pi = iln(e) = ln(-1) = ln(e^i)
   e^sqrt(-1) = e^i = e^ln(e^i) =>
   sqrt(-n) = sqrt(n)*i = sqrt(n)*ln(e^i) =>
   e^sqrt(-1) = e^i = +/- 1 = sqrt(1)
   sqrt(n) = e^sqrt(-n)
   sqrt(n) = e^i\*sqrt(n) =>
   sqrt(1/4) = 1/2
   sqrt(-1/4) = e^sqrt(1/4) = e^i\*sqrt(-1/4) = +/- sqrt(-1/4) = +/- isqrt(1/4)
   = +/- i1/2 =>
   sqrt(n) = e^sqrt(-n) = e^i\*sqrt(n) = +/- sqrt(n)
   sqrt(-n) = +/- isqrt(n)
1. i hypothesis (i is an irrational number)
   e^i = cos(1) + isin(1) = +/- 1 = 0.54030230586 + isin(1) =>
   isin(1) = 0.45969769414 or -1.54030230586
   sin(1) = 0.8414709848
   i = 0.45969769414 / 0.8414709848 or -1.54030230586 / 0.8414709848
   i = 0.54630248985 or -1.83048772172
   +/- ln(e) = 2ei = 1 or 2 or 3 = +/> 2
   e^i + ei = 1(ln(e)) or 2 or 3 = +/> 2
   +/> 0 = 0 or 1 or -1 = (+/> 1)\*(0)
   +/> 0 = +/> 1 \* 0 = 0 or +/> 0 , since (1)
   (*1) x = 0 = x*0 = 0\*0 = 0 ! thus,
   +>x = +/- x or +/- (x-1) or +/- (x+1) or 0
   so, +>x can return a set of either 3,5 or 7 numbers

golden ratio p

p = (1+sqrt(5))/2
let p' = (1+sqrt(-5))/2 then,
p' |=| x |=| p' |=| 1+sqrt(-5) |=| 2x
|=| sqrt(-5) |=| 2x - 1
sqrt(-5) |=| +/- i(sqrt(5))
+/- i |=| (2x-1)/sqrt(5)
+/- i |=| sqrt(-5)/sqrt(5)
|=| +/- i sqrt(5)/sqrt(5) |=| +/- i
so, +/- i = sqrt(-x)/sqrt(x) ?

sqrt(n) = e^sqrt(-n) = e^i \* sqrt(n) ?

by S i mean integral.
S(2e^2)dx = 2e^2x + c = c + 2xei = c + 2(+>x) ERROR
so, e^2x = +>x and +>x = xei thus, +>x is an imaginary component
this means that 2(+>x) + c requires reductive proofs to be able to be related to algebra "R-Algebra"
+>x + +>x = xe^2 + xe^2 = 2xe^2 = 2+>x

sqrt(n) = +/-sqrt(-1)+/-sqrt(-1)sqrt(n)

= sqrt(-1)sqrt(-n)
= isqrt(-n)
= e^sqrt(n) = e^(i\*sqrt(-n))
= sqrt(n)ie^i

then, ie^i = 1 ?

hypothesis 2(+>i) = (+>i)^2 (INCORRECT):

+>i + +>i =
{-2i-2,-2i-1,-2i,-2i+1,-2i+2} +
{-i-1,-i,-i+1} +
{-2,-1,0,1,2} +
{2i-2,2i-1,2i,2i+1,2i+2} +
{i-1,i,i+1}

(+>i)^2 = {-2,-1,0,1,2} + {?} + {-2i-2} NOTEQ 2(+>i)
